Worked on the patterns

Charge!/src/Charge/Tactics/Rtac/Red.v
@@ -1,3 +1,6 @@
+Require Import ExtLib.Structures.Applicative.
+Require Import ExtLib.Core.RelDec.
+
 Require Import Charge.Views.ILogicView.
 Require Import Charge.Patterns.ILogicPattern.
 Require Import Charge.Views.BILogicView.
@@ -6,6 +9,8 @@ Require Import Charge.Views.EmbedView.
 Require Import Charge.Patterns.EmbedPattern.
 
 Require Import MirrorCore.Lambda.ExprCore.
+Require Import MirrorCore.Lambda.ExprLift.
+Require Import MirrorCore.Lambda.Ptrns.
 Require Import MirrorCore.CTypes.CoreTypes.
 Require Import MirrorCore.Views.Ptrns.
 Require Import MirrorCore.Lib.ApplicativeView.
@@ -23,32 +28,82 @@ Section Red.
   Context {FVEmbed : PartialView func (embed_func typ)}.
   Context {FVAp : PartialView func (ap_func typ)}.
   Context {Expr_expr : Expr typ (expr typ func)}.
+  Context {RSym_func : RSym func}.
+  Context {T : Type -> Type} {Applicative_T : Applicative T}.
 
-  Definition pointwise_redF (f : typ -> expr typ func -> expr typ func) (g : typ -> typ) : 
-    ptrn (expr typ func) (expr typ func)  :=
+  Context {Typ1_T : Typ1 _ T}.
+  Let g := @typ1 _ _ T _.
+
+
+  Definition pointwise_redF (tus tvs : tenv typ)
+    (f : tenv typ -> tenv typ -> typ -> expr typ func -> typ * expr typ func) :
+    ptrn (expr typ func) (typ * expr typ func)  :=
     Eval compute in 
-      por (bil_pointwise_red f g) 
-          (por (embed_pointwise_red f g) 
-               (por (red_ap_ptrn f)
-                    (il_pointwise_red f g))).
+      por (bil_pointwise_red (f tus tvs) g) 
+          (por (embed_pointwise_red (f tus tvs) g) 
+               (por (red_ap_ptrn (f tus tvs))
+                    (il_pointwise_red tus tvs f g))).
+          
+  Fixpoint pointwise_red_aux 
+      (s : expr typ func) 
+      (tus tvs : tenv typ) (t : typ) (e : expr typ func) {struct e} : 
+        typ * expr typ func :=
+    let f := pointwise_red_aux s in
+    run_ptrn (pointwise_redF tus tvs f)
+             (t, App e (lift 0 (length tvs) s)) e.
 
-  Fixpoint pointwise_red_aux (s : expr typ func) (g : typ -> typ) (t : typ) (e : expr typ func) {struct e} : expr typ func :=
-    run_ptrn (pointwise_redF (pointwise_red_aux s g) g) (App e s) e.
-
-  Definition pointwise_red (t : typ) (s e : expr typ func) (g : typ -> typ) := pointwise_red_aux s g t e.
+  Definition pointwise_red (t : typ) (s e : expr typ func) := 
+    pointwise_red_aux s nil nil t e.
 
   Definition red_entails_lhs (g : typ -> typ) :=
     pmap (fun t' => let '(t, (p, s), r) := t' in 
-    		 mkEntails t (pointwise_red t s p g) r)
+    		 mkEntails t (snd (pointwise_red t s p)) r)
          (ptrnEntails get (Ptrns.app get get) get).
 
   Definition RED_ENTAILS (g : typ -> typ) : rtac typ (expr typ func) :=
     fun c s e =>
       run_ptrn (pmap (fun e' => More s (GGoal e')) (red_entails_lhs g)) Fail e.
       
-  Lemma RED_ENTAILS_sound (g : typ -> typ) : rtac_sound (RED_ENTAILS g).
+  Lemma RED_ENTAILS_sound : rtac_sound (RED_ENTAILS g).
   Proof.
     admit.
   Admitted.
+
+  Definition pointwise_restoreF (tus tvs : tenv typ) (s : expr typ func) (t : typ) 
+    (f : tenv typ -> tenv typ -> typ -> expr typ func -> typ * expr typ func) : 
+    ptrn (expr typ func) (typ * expr typ func)  :=
+    Eval compute in 
+      por (bil_pointwise_red (f tus tvs) g) 
+          (por (embed_pointwise_red (f tus tvs) g)                
+               (il_pointwise_red tus tvs f g)).
+SearchAbout RelDec ctyp.                         
+
+  Fixpoint pointwise_restore_aux 
+      (s : expr typ func) 
+      (g : typ -> typ) 
+      (tus tvs : tenv typ) (t : typ) (e : expr typ func) {struct e} : 
+        typ * expr typ func :=
+    let f := pointwise_restore_aux s g in
+    let default := run_ptrn (por (restore_ap_ptrn tus tvs s (f tus tvs t)) (restore_pure_ptrn tus tvs)) (t, e) e in
+    run_ptrn (pointwise_restoreF tus tvs s t f)
+             default e.
+
+  Definition pointwise_restore (t : typ) (s e : expr typ func) := 
+    pointwise_restore_aux s g nil nil t e.
+
+  Definition restore_entails_lhs (s : expr typ func) :=
+    pmap (fun t' => let '(t, p, r) := t' in 
+    		 mkEntails t (snd (pointwise_restore t s p)) r)
+         (ptrnEntails get get get).
+
+  Definition RESTORE_ENTAILS (s : expr typ func) : rtac typ (expr typ func) :=
+    fun c s' e =>
+      run_ptrn (pmap (fun e' => More s' (GGoal e')) (restore_entails_lhs s)) Fail e.
+  
+  Lemma RESTORE_ENTAILS_sound (s : expr typ func) : rtac_sound (RESTORE_ENTAILS s). 
+  Proof.
+    admit.
+  Admitted.
+
 
 End Red.
