Charge!/src/Charge/Patterns/EmbedPattern.v
@@ -72,9 +72,10 @@ Section EmbedPointwiseRed.
   Context {typ func : Set} {FV : PartialView func (embed_func typ)}.
 
   Definition embed_pointwise_red
-    (f : typ -> expr typ func -> expr typ func) 
+    (f : typ -> expr typ func -> typ * expr typ func) 
     (g : typ -> typ) :=
-      pmap (fun t_u_p => let '(t, u, p) := t_u_p in mkEmbed (g t) (g u) (f u p))
+      pmap (fun t_u_p => let '(t, u, p) := 
+        t_u_p in (t, mkEmbed (g t) (g u) (snd (f u p))))
            (ptrnEmbed get get).
 
 End EmbedPointwiseRed.
